SP1Foundations.lean
@@ -2,5 +2,6 @@ import SP1Foundations.ByteOpcode
 import SP1Foundations.Constraint
 import SP1Foundations.Field
 import SP1Foundations.Misc
+import SP1Foundations.SailM
 import SP1Foundations.Unsigned
 import SP1Foundations.Word
